@prefix dc: <http://purl.org/dc/elements/1.1/> .
@prefix gic: <http://www.cngl.ie/ontologies/gicup#> .
@prefix gicd: <http://www.cngl.ie/ontologies/gic_domain#> .
@prefix its: <http://www.w3.org/International/multilingualweb/lt#> .
@prefix nif: <http://persistance.uni-leipzig.org/nlp2rdf/ontologies/nif-core#> .
@prefix owl: <http://www.w3.org/2002/07/owl#> .
@prefix prov: <http://www.w3.org/ns/prov#> .
@prefix rdf: <http://www.w3.org/1999/02/22-rdf-syntax-ns#> .
@prefix rdfs: <http://www.w3.org/2000/01/rdf-schema#> .
@prefix sso: <http://nlp2rdf.lod2.eu/schema/sso#> .
@prefix str: <http://nlp2rdf.lod2.eu/schema/str> .
@prefix xsd: <http://www.w3.org/2001/XMLSchema#> .

str:String rdfs:subClassOf gic:Content .

gicd: a owl:Ontology;
   rdfs:label "Global Intelligent Content Semantic Model - Domain Specific Part";
   dc:contributor "Alan Meehan",
     "Eamonn Kenny",
     "Ergun Bicici",
     "Erwin Moreau",
     "Leroy Finn",
     "Joachim Wagner",
     "Joao Cabral",
     "Martin Emms",
     "Melike Sah",
     "M. Rami Ghorab",
     "Nick Campbell",
     "Qun Liu",
     "Xiaofeng Wu",
     "Xiaojun Zhang";
   dc:creator "Rob Brennan",
     "David Lewis";
   dc:date "2014-05-01";
   dc:description "This semantic model contain domain-specific elements that extend the basic global Intelligent Content Model in experimental ways";
   dc:rights "The ontology license is the Creative Commons Attribution License - http://creativecommons.org/licenses/by/3.0 .";
   dc:title "Global Intelligent Content Semantic Model - Domain Specific Part";
   rdfs:comment "The model is expressed in OWL2-RL encoded as Turtle/RDF with embedded definitions describing the concepts and relationships that make up the model. ";
   owl:imports gic:;
   owl:versionIRI <http://www.cngl.ie/ontologies/gic_domain/0.3.0#>;
   owl:versionInfo "0.3.0" .

gicd:AnalysedText a owl:Class;
   rdfs:label "AnalysedText";
   rdfs:comment "a string identified by some text analysis process as possessing some common semantic and/or lexical characteristics.";
   rdfs:subClassOf gic:Content .

gicd:Extraction a owl:Class;
   rdfs:label "Extraction";
   rdfs:comment "The process of extracting translatable text from some source content for the purposes of translation.";
   rdfs:subClassOf gic:ContentProcessingActivity;
   owl:equivilentClass [
     a owl:Restriction;
     owl:allValuesFrom [ owl:unionOf (gic:Content)];
     owl:onProperty gic:contentConsumed
   ],  [
     a owl:Restriction;
     owl:allValuesFrom [ owl:unionOf (gic:Content gicd:SourceUnit)];
     owl:onProperty gic:contentGenerated
   ] .

gicd:Merging a owl:Class;
   rdfs:label "Merging";
   rdfs:comment "Merging is the integration of translated content into a completed target language document format.";
   rdfs:subClassOf prov:Activity .

gicd:Person a owl:Class;
   rdfs:label "Person";
   rdfs:comment "A person in the real world that interacts with global intelligent content.";
   rdfs:subClassOf prov:Agent .

gicd:Project a owl:Class;
   rdfs:label "Project";
   rdfs:comment "Project is the representation of a localisation project within an organisational domain. It is annotated with the details and resources  typically found in a TIPP manifest, including the project meta-data expressed in a Linport descriptor. ";
   rdfs:subClassOf prov:Entity .

gicd:QualityReview a owl:Class;
   rdfs:label "QualityReview";
   rdfs:comment "The assessment of the linguistic quality of a translation considering both the translation, revised translation or source. Its may also be applied to any of the source content.";
   rdfs:subClassOf gic:ContentProcessingActivity;
   owl:equivilentClass [
     a owl:Restriction;
     owl:allValuesFrom [ owl:unionOf (gic:Content gicd:SourceUnit gicd:Segment gicd:Term nif:String nif:Structure nif:Word nif:Phrase sso:Word sso:Phrase gicd:Translation gicd:TranslationRevision)];
     owl:onProperty gic:contentConsumed
   ],  [
     a owl:Restriction;
     owl:allValuesFrom [ owl:unionOf (gic:Content gicd:QualityAssessment)];
     owl:onProperty gic:contentGenerated
   ] .

gicd:ReviseTranslation a owl:Class;
   rdfs:label "ReviseTranslation";
   rdfs:comment "The change of a translation after consideration of the translation and the corresponding source content.";
   rdfs:subClassOf gic:ContentProcessingActivity;
   owl:equivilentClass [
     a owl:Restriction;
     owl:allValuesFrom [ owl:unionOf (gic:Content gicd:SourceUnit gicd:Segment gicd:Term nif:String nif:Structure nif:Word nif:Phrase sso:Word sso:Phrase gicd:Translation gicd:TranslationRevision)];
     owl:onProperty gic:contentConsumed
   ],  [
     a owl:Restriction;
     owl:allValuesFrom [ owl:unionOf (gic:Content gicd:TranslationRevision)];
     owl:onProperty gic:contentGenerated
   ] .

gicd:Segmentation a owl:Class;
   rdfs:label "Segmentation";
   rdfs:comment "The subdividing source content to a granularity designed to ease  translation.";
   rdfs:subClassOf gic:ContentProcessingActivity;
   owl:equivilentClass [
     a owl:Restriction;
     owl:allValuesFrom [ owl:unionOf (gic:Content gicd:SourceUnit)];
     owl:onProperty gic:contentConsumed
   ],  [
     a owl:Restriction;
     owl:allValuesFrom [ owl:unionOf (gic:Content gicd:Segment)];
     owl:onProperty gic:contentGenerated
   ] .

gicd:TerminologyIdentification a owl:Class;
   rdfs:label "Terminology Identification";
   rdfs:comment "The identification of Terms that should be subject to consistent translation, derived from Word or Phrases service by Text Analysis or directly from Segments or Source Units.";
   rdfs:subClassOf gic:ContentProcessingActivity;
   owl:equivilentClass [
     a owl:Restriction;
     owl:allValuesFrom [ owl:unionOf (gic:Content nif:String nif:Structure nif:Word nif:Phrase nif:Sentence sso:Phrase sso:Word)];
     owl:onProperty gic:contentConsumed
   ],  [
     a owl:Restriction;
     owl:allValuesFrom [ owl:unionOf (gic:Content gicd:Term)];
     owl:onProperty gic:contentGenerated
   ] .

gicd:TextAnalysis a owl:Class;
   rdfs:label "TextAnalysis";
   rdfs:comment "Text analysis involves information retrieval, lexical analysis to study word frequency distributions, pattern recognition, tagging/annotation, information extraction, data mining techniques including link and association analysis, visualization, and predictive analytics. The overarching goal is, essentially, to turn text into data for analysis, via application of natural language processing (NLP) and analytical methods (Wikipedia).";
   rdfs:subClassOf gicd:ContentProcessingActivity;
   owl:equivilentClass [
     a owl:Restriction;
     owl:allValuesFrom [ owl:unionOf (gic:Content nif:String nif:Structure nif:Word nif:Phrase nif:Sentence)];
     owl:onProperty gic:contentConsumed
   ],  [
     a owl:Restriction;
     owl:allValuesFrom [ owl:unionOf (gic:Content nif:String nif:Phrase nif:Word sso:Phrase sso:Word)];
     owl:onProperty gic:contentGenerated
   ] .

gicd:Translate a owl:Class;
   rdfs:label "Translate";
   rdfs:comment "The translation of any source content, including Source Unit, Segment, Term, Word or Phrase into a target language.";
   rdfs:subClassOf gic:ContentProcessingActivity;
   owl:equivilentClass [
     a owl:Restriction;
     owl:allValuesFrom [ owl:unionOf (gic:Content gicd:SourceUnit gicd:Segment gicd:Term nif:String nif:Structure nif:Word nif:Phrase sso:Word sso:Phrase)];
     owl:onProperty gic:contentConsumed
   ],  [
     a owl:Restriction;
     owl:allValuesFrom [ owl:unionOf (gic:Content gicd:Translation)];
     owl:onProperty gic:contentGenerated
   ] .

gicd:wasAssessmentOf a owl:ObjectProperty;
   rdfs:label "wasAssessmentOf";
   rdfs:comment "Links some Content to a Quality Assessment.";
   rdfs:domain gic:Content;
   rdfs:range gicd:QualityAssessment;
   rdfs:subPropertyOf prov:wasDerivedFrom .

gicd:wasTranslatedFrom a owl:ObjectProperty;
   rdfs:label "wasTranslatedFrom";
   rdfs:comment "Links a gicd:Translation (as range) to the corresponding source text.";
   rdfs:domain gic:Content;
   rdfs:range gicd:Translation;
   rdfs:subPropertyOf prov:wasDerivedFrom .

gicd:QualityAssessment a owl:Class;
   rdfs:label "QualityAssessment";
   rdfs:comment "For the assessing the quality of localised content";
   rdfs:subClassOf its:localisationQualityIssue .

gicd:TranslationRevision a owl:Class;
   rdfs:label "TranslationRevision";
   rdfs:comment "the revision of a string that was originally a Translation";
   rdfs:subClassOf gic:Content .

gicd:Segment a owl:Class;
   rdfs:label "Segment";
   rdfs:comment "A string resulting from subdividing source content to a granularity designed to ease translation. Typically this is a sentence, but may also be text from a heading  cell or a table.";
   rdfs:subClassOf gic:Content .

gicd:Term a owl:Class;
   rdfs:label "Term";
   rdfs:comment "A string that is subject to terminology management with the intention of supporting consistent source content and the consistent translation  the source term.";
   rdfs:subClassOf gic:Content .

gicd:Translation a owl:Class;
   rdfs:label "Translation";
   rdfs:comment "A string that was produced by translating another string from its source language into a specified target language";
   rdfs:subClassOf gic:Content .

gicd:SourceUnit a owl:Class;
   rdfs:label "SourceUnit";
   rdfs:comment "a string extracted from a source document for the purposes of translating the text it contains.";
   rdfs:subClassOf gic:Content .